New SHA_helpers interface that doesn't depend on SHA specs or UInt*

vale/code/crypto/sha/SHA_helpers.fsti
@@ -2,14 +2,10 @@ module SHA_helpers
 
 open Prop_s
 open Opaque_s
-open Spec.SHA2
-open Spec.Hash
-open Spec.Hash.Helpers
 open X64.CryptoInstructions_s
 open Types_s
 open Words_s
 open FStar.Seq
-open FStar.UInt32  // Interop with UInt-based SHA spec
 open Arch.Types
 
 unfold
@@ -17,143 +13,134 @@ let (.[]) = FStar.Seq.index
 
 #reset-options "--max_fuel 0 --max_ifuel 0"
   
-// Define these specific converters here, so that F* only reasons about 
-// the correctness of the conversion once, rather that at every call site
-let vv (u:UInt32.t) : nat32 = v u
-let to_uint32 (n:nat32) : UInt32.t = uint_to_t n
-
-// Duplicate these definitions from Spec.SHA2.fst, since we can't see it here
-let block_w  (a: sha2_alg) = m:seq (word a) {length m = size_block_w}
+// Specialize these definitions (from Spec.SHA2.fst) for SHA256
+unfold let size_k_w = 64
+val word:Type0
+unfold let size_hash_w =8
+(* Number of words for a block size *)
+let size_block_w = 16
+(* Define the size block in bytes *)
+let size_block =
+  let open FStar.Mul in
+  4 (*size_word a*) * size_block_w
+let block_w  = m:seq word {length m = size_block_w}
 let counter = nat
-val k0 : (seq (word SHA2_256) {length k0 = 64}
- 
+val k0 : (s:seq word {length s = size_k_w})
+unfold let hash256 = m:Seq.seq word {Seq.length m = size_hash_w}
+
+(* Input data. *)
+val byte:Type0
+type bytes =  m:Seq.seq byte
+
+(* Input data, multiple of a block length. *)
+let bytes_blocks =
+  l:bytes { Seq.length l % size_block = 0 }
+
 // Hide various SHA2 definitions
-val ws_opaque (a:sha2_alg) (b:block_w a) (t:counter{t < 64}): Tot (word a)
-val shuffle_core_opaque (a:sha2_alg) (block:block_w a) (hash:hash_w a) (t:counter{t < 64}): Tot (hash_w a) 
-val update_multi_opaque (a:hash_alg) (hash:hash_w a) (blocks:bytes_blocks a):Tot (hash_w a) (decreases (length blocks))
+val ws_opaque (b:block_w) (t:counter{t < size_k_w}): Tot (nat32)
+val shuffle_core_opaque (block:block_w) (hash:hash256) (t:counter{t < size_k_w}): Tot (hash256) 
+val update_multi_opaque (hash:hash256) (blocks:bytes_blocks):Tot (hash256) 
+
+// Hide some functions that operate on words & bytes
+val add_mod (x:word) (y:nat32) : nat32
+val word_to_nat32 (x:word) : nat32
+val nat32_to_word (x:nat32) : word
+val byte_to_nat8 (b:byte) : nat8
+val nat8_to_byte (b:nat8) : byte
 
 // Work around some limitations in Vale's support for dependent types
-unfold let block256 = block_w SHA2_256
-unfold let hash256 = hash_w SHA2_256
+
 //unfold let bytes_blocks256 = bytes_blocks SHA2_256
-unfold let repeat_range_vale (max:nat { max < 64}) (block:block256) (hash:hash256) =
-  Spec.Loops.repeat_range 0 max (shuffle_core_opaque SHA2_256 block) hash
-unfold let lemma_repeat_range_0_vale (block:block256) (hash:hash256) = 
-  Spec.Loops.repeat_range_base 0 (shuffle_core_opaque SHA2_256 block) hash
+unfold let repeat_range_vale (max:nat { max < size_k_w}) (block:block_w) (hash:hash256) =
+  Spec.Loops.repeat_range 0 max (shuffle_core_opaque block) hash
+unfold let lemma_repeat_range_0_vale (block:block_w) (hash:hash256) = 
+  Spec.Loops.repeat_range_base 0 (shuffle_core_opaque block) hash
 unfold let update_multi_opaque_vale (hash:hash256) (blocks:bytes) : hash256 = 
-  if length blocks % 64 = 0 then let b:bytes_blocks SHA2_256 = blocks in update_multi_opaque SHA2_256 hash b else hash
+  if length blocks % size_k_w = 0 then let b:bytes_blocks = blocks in update_multi_opaque hash b else hash
 
-val make_hash_def (abef cdgh:quad32) :
-    (hash:hash_w SHA2_256 {
-         length hash == 8 /\
-         hash.[0] == to_uint32 abef.hi3 /\
-         hash.[1] == to_uint32 abef.hi2 /\
-         hash.[2] == to_uint32 cdgh.hi3 /\
-         hash.[3] == to_uint32 cdgh.hi2 /\
-         hash.[4] == to_uint32 abef.lo1 /\
-         hash.[5] == to_uint32 abef.lo0 /\
-         hash.[6] == to_uint32 cdgh.lo1 /\
-         hash.[7] == to_uint32 cdgh.lo0    
-    } ) 
 
-unfold let make_hash = make_opaque make_hash_def
-
-val make_ordered_hash_def (abcd efgh:quad32) :
-  (hash:hash_w SHA2_256 {
-         length hash == 8 /\
-         hash.[0] == to_uint32 abcd.lo0 /\
-         hash.[1] == to_uint32 abcd.lo1 /\
-         hash.[2] == to_uint32 abcd.hi2 /\
-         hash.[3] == to_uint32 abcd.hi3 /\
-         hash.[4] == to_uint32 efgh.lo0 /\
-         hash.[5] == to_uint32 efgh.lo1 /\
-         hash.[6] == to_uint32 efgh.hi2 /\
-         hash.[7] == to_uint32 efgh.hi3      
-   })
-   
-unfold let make_ordered_hash = make_opaque make_ordered_hash_def
+val make_hash (abef cdgh:quad32) : hash256
+val make_ordered_hash (abef cdgh:quad32): hash256
 
 // Top-level proof for the SHA256_rnds2 instruction
-val lemma_sha256_rnds2 (abef cdgh xmm0:quad32) (t:counter) (block:block_w SHA2_256) (hash_in:hash_w SHA2_256) : Lemma
-  (requires t + 1 < 64 /\
-            xmm0.lo0 == add_wrap (vv (k0 SHA2_256).[t]  ) (vv (ws_opaque SHA2_256 block t)) /\
-            xmm0.lo1 == add_wrap (vv (k0 SHA2_256).[t+1]) (vv (ws_opaque SHA2_256 block (t+1))) /\ 
-            make_hash abef cdgh == Spec.Loops.repeat_range_spec 0 t (shuffle_core_opaque SHA2_256 block) hash_in
+val lemma_sha256_rnds2 (abef cdgh xmm0:quad32) (t:counter) (block:block_w) (hash_in:hash256) : Lemma
+  (requires t + 1 < size_k_w /\
+            xmm0.lo0 == add_mod k0.[t]   (ws_opaque block t) /\
+            xmm0.lo1 == add_mod k0.[t+1] (ws_opaque block (t+1)) /\ 
+            make_hash abef cdgh == Spec.Loops.repeat_range 0 t (shuffle_core_opaque block) hash_in
             )
   (ensures make_hash (sha256_rnds2_spec cdgh abef xmm0) abef ==
-           Spec.Loops.repeat_range_spec 0 (t+2) (shuffle_core_opaque SHA2_256 block) hash_in)
+           Spec.Loops.repeat_range 0 (t+2) (shuffle_core_opaque block) hash_in)
 
 (* Proof work for the SHA256_msg* instructions *)
-let ws_quad32 (t:counter) (block:block_w SHA2_256) : quad32 =
-    if t < 64 - 3 then
-       Mkfour (vv (ws_opaque SHA2_256 block t))
-              (vv (ws_opaque SHA2_256 block (t+1)))
-              (vv (ws_opaque SHA2_256 block (t+2)))
-              (vv (ws_opaque SHA2_256 block (t+3)))
+let ws_quad32 (t:counter) (block:block_w) : quad32 =
+    if t < size_k_w - 3 then
+       Mkfour (ws_opaque block t)
+              (ws_opaque block (t+1))
+              (ws_opaque block (t+2))
+              (ws_opaque block (t+3))
     else 
        Mkfour 0 0 0 0
 
-
-val ws_partial_def (t:counter) (block:block_w SHA2_256) : quad32
+val ws_partial_def (t:counter) (block:block_w) : quad32
 unfold let ws_partial = make_opaque ws_partial_def
 
 // Top-level proof for the SHA256_msg1 instruction
-val lemma_sha256_msg1 (dst src:quad32) (t:counter) (block:block_w SHA2_256) : Lemma
-  (requires 16 <= t /\ t < 64 /\
+val lemma_sha256_msg1 (dst src:quad32) (t:counter) (block:block_w) : Lemma
+  (requires 16 <= t /\ t < size_k_w /\
             dst == ws_quad32 (t-16) block /\
-            src.lo0 == vv(ws_opaque SHA2_256 block (t-12)))
+            src.lo0 == ws_opaque block (t-12))
   (ensures sha256_msg1_spec dst src == ws_partial t block)
 
   
 // Top-level proof for the SHA256_msg2 instruction
-val lemma_sha256_msg2 (src1 src2:quad32) (t:counter) (block:block_w SHA2_256) : Lemma
-  (requires 16 <= t /\ t < 64 - 3 /\
+val lemma_sha256_msg2 (src1 src2:quad32) (t:counter) (block:block_w) : Lemma
+  (requires 16 <= t /\ t < size_k_w - 3 /\
             (let step1 = ws_partial t block in
              let t_minus_7 = ws_quad32 (t-7) block in
              src1 == add_wrap_quad32 step1 t_minus_7 /\
 
-             src2.hi2 == vv (ws_opaque SHA2_256 block (t-2)) /\
-             src2.hi3 == vv (ws_opaque SHA2_256 block (t-1))))
+             src2.hi2 == ws_opaque block (t-2) /\
+             src2.hi3 == ws_opaque block (t-1)))
   (ensures sha256_msg2_spec src1 src2 == ws_quad32 t block)
 
 open Workarounds
 
 (* Abbreviations and lemmas for the code itself *)
 let k_reqs (k_seq:seq quad32) : prop0 =
-  length k_seq == 64 / 4 /\
-  (forall i . {:pattern (index_work_around_quad32 k_seq i)} 0 <= i /\ i < (64/4) ==> 
-    (k_seq.[i]).lo0 == vv (k0 SHA2_256).[4 `op_Multiply` i] /\
-    (k_seq.[i]).lo1 == vv (k0 SHA2_256).[4 `op_Multiply` i + 1] /\
-    (k_seq.[i]).hi2 == vv (k0 SHA2_256).[4 `op_Multiply` i + 2] /\
-    (k_seq.[i]).hi3 == vv (k0 SHA2_256).[4 `op_Multiply` i + 3])
+  length k_seq == size_k_w / 4 /\
+  (forall i . {:pattern (index_work_around_quad32 k_seq i)} 0 <= i /\ i < (size_k_w/4) ==> 
+    (k_seq.[i]).lo0 == word_to_nat32 (k0.[4 `op_Multiply` i]) /\
+    (k_seq.[i]).lo1 == word_to_nat32 (k0.[4 `op_Multiply` i + 1]) /\
+    (k_seq.[i]).hi2 == word_to_nat32 (k0.[4 `op_Multiply` i + 2]) /\
+    (k_seq.[i]).hi3 == word_to_nat32 (k0.[4 `op_Multiply` i + 3]))
   
-let quads_to_block (qs:seq quad32) : block_w SHA2_256
+let quads_to_block (qs:seq quad32) : block_w
   =
   let nat32_seq = Words.Seq_s.seq_four_to_seq_LE qs in
-  let f (n:nat{n < 16}) : UInt32.t = to_uint32 (if n < length nat32_seq then nat32_seq.[n] else 0) in
+  let f (n:nat{n < 16}) : word = nat32_to_word (if n < length nat32_seq then nat32_seq.[n] else 0) in
   init 16 f
 
 val lemma_quads_to_block (qs:seq quad32) : Lemma
   (requires length qs == 4)
   (ensures (let block = quads_to_block qs in
             forall i . {:pattern (index_work_around_quad32 qs i)} 0 <= i /\ i < 4 ==>
-              (qs.[i]).lo0 == vv (ws_opaque SHA2_256 block (4 `op_Multiply` i + 0)) /\
-              (qs.[i]).lo1 == vv (ws_opaque SHA2_256 block (4 `op_Multiply` i + 1)) /\
-              (qs.[i]).hi2 == vv (ws_opaque SHA2_256 block (4 `op_Multiply` i + 2)) /\
-              (qs.[i]).hi3 == vv (ws_opaque SHA2_256 block (4 `op_Multiply` i + 3)) /\
+              (qs.[i]).lo0 == ws_opaque block (4 `op_Multiply` i + 0) /\
+              (qs.[i]).lo1 == ws_opaque block (4 `op_Multiply` i + 1) /\
+              (qs.[i]).hi2 == ws_opaque block (4 `op_Multiply` i + 2) /\
+              (qs.[i]).hi3 == ws_opaque block (4 `op_Multiply` i + 3) /\
               qs.[i] == ws_quad32 (4 `op_Multiply` i) block))
          
-val update_block (hash:hash256) (block:block256): Tot (hash256)
+val update_block (hash:hash256) (block:block_w): hash256
 
-val update_lemma (src1 src2 src1' src2' h0 h1:quad32) (block:block_w SHA2_256) : Lemma
+val update_lemma (src1 src2 src1' src2' h0 h1:quad32) (block:block_w) : Lemma
   (requires (let hash_orig = make_hash h0 h1 in
              make_hash src1 src2 == 
-             Spec.Loops.repeat_range_spec 0 64 (shuffle_core_opaque SHA2_256 block) hash_orig /\
+             Spec.Loops.repeat_range 0 size_k_w (shuffle_core_opaque block) hash_orig /\
              src1' == add_wrap_quad32 src1 h0 /\
              src2' == add_wrap_quad32 src2 h1))
   (ensures (let hash_orig = make_hash h0 h1 in
             make_hash src1' src2' == update_block hash_orig block))
-
 
 let rec update_multi_quads (s:seq quad32) (hash_orig:hash256) : Tot (hash256) (decreases (length s))
   =
@@ -165,24 +152,23 @@ let rec update_multi_quads (s:seq quad32) (hash_orig:hash256) : Tot (hash256) (d
     let hash = update_block h_prefix (quads_to_block qs) in
     hash
 
-let seq_nat8_to_seq_U8 (b:seq nat8) : (b':seq UInt8.t) =
-  init (length b) (fun (i:nat { i < length b }) -> let x:UInt8.t = UInt8.uint_to_t (index b i) in x)
+let seq_nat8_to_seq_byte (b:seq nat8) : (b':seq byte) =
+  init (length b) (fun (i:nat { i < length b }) -> let x:byte = nat8_to_byte (index b i) in x)
 
 
-val lemma_update_multi_equiv_vale (hash hash':hash_w SHA2_256) (quads:seq quad32) (r_quads:seq quad32)
-  (nat8s:seq nat8) (blocks:seq UInt8.t) :
+val lemma_update_multi_equiv_vale (hash hash':hash256) (quads:seq quad32) (r_quads:seq quad32)
+  (nat8s:seq nat8) (blocks:seq byte) :
   Lemma (requires length quads % 4 == 0 /\
                   r_quads == reverse_bytes_quad32_seq quads /\
                   nat8s == le_seq_quad32_to_bytes quads /\
-                  blocks == seq_nat8_to_seq_U8 nat8s /\
+                  blocks == seq_nat8_to_seq_byte nat8s /\
                   hash' == update_multi_quads r_quads hash)        
         (ensures 
-           length blocks % 64 == 0 /\
+           length blocks % size_k_w == 0 /\
            hash' == update_multi_opaque_vale hash blocks)
         (decreases (length quads)) 
 
-
-val lemma_update_multi_quads (s:seq quad32) (hash_orig:hash_w SHA2_256) (bound:nat) : Lemma
+val lemma_update_multi_quads (s:seq quad32) (hash_orig:hash256) (bound:nat) : Lemma
     (requires bound + 4 <= length s)
     (ensures (let prefix_LE = slice s 0 bound in
               let prefix_BE = reverse_bytes_quad32_seq prefix_LE in
@@ -194,13 +180,13 @@ val lemma_update_multi_quads (s:seq quad32) (hash_orig:hash_w SHA2_256) (bound:n
               let h = update_block h_prefix (quads_to_block block_quads_BE) in
               h == update_multi_quads input_BE hash_orig))
 
-let le_bytes_to_hash (b:seq nat8) : hash_w SHA2_256 =
+let le_bytes_to_hash (b:seq nat8) : hash256 =
   if length b <> 32 then   
-     (let f (n:nat{n < 8}) : UInt32.t = to_uint32 0 in
+     (let f (n:nat{n < 8}) : word = nat32_to_word 0 in
      init 8 f)
   else (
      let open Words.Seq_s in
-     Spec.Loops.seq_map to_uint32 (seq_nat8_to_seq_nat32_LE b)
+     Spec.Loops.seq_map nat32_to_word (seq_nat8_to_seq_nat32_LE b)
   )
 
 val lemma_hash_to_bytes (s:seq quad32) : Lemma
